coq: ZF: Meta: refactor

coq/ZF/Meta/Term/HasTy.v
@@ -2,94 +2,92 @@ Require Import Coq.Lists.List.
 Require Import Coq.Strings.String.
 
 Require Import ZF.Meta.Ctx.
-Require Import ZF.Meta.Sigs.
+Require Import ZF.Meta.Env.
 Require Import ZF.Meta.Term.Syntax.
 Require Import ZF.Meta.Ty.
 
 Import ListNotations.
 
-Inductive HasTy (S:Sigs) : Ctx -> Term -> Ty -> Prop :=
+Inductive HasTy (E:Env) : Ctx -> Term -> Ty -> Prop :=
 | HasTyBot : forall (G:Ctx),
-    HasTy S G Bot TyProp
+    HasTy E G Bot TyProp
 | HasTyTop : forall (G:Ctx),
-    HasTy S G Top TyProp
+    HasTy E G Top TyProp
 | HasTyVar : forall (G:Ctx) (n:nat) (ty:Ty),
-    typeOf G n = Some ty ->
-    HasTy S G (Var n) ty
-| HasTyIdent : forall (G:Ctx) (name:string) (args:list Term)
-    (argTys:list Ty) (ty:Ty),
-    S name = Some (argTys, ty) ->
-    HasTys S G args argTys ->
-    HasTy S G (Ident name args) ty
+    typeOf G n = Some ty                    ->
+    HasTy E G (Var n) ty
+| HasTyIdent : forall (G:Ctx) (name:string) (args:list Term) (tys:list Ty) (ty:Ty),
+    Env.toSigs E name = Some (tys, ty)      ->
+    HasTys E G args tys                     ->
+    HasTy E G (Ident name args) ty
 | HasTyElem : forall (G:Ctx) (x y:Term),
-    HasTy S G x TySet ->
-    HasTy S G y TySet ->
-    HasTy S G (Elem x y) TyProp
+    HasTy E G x TySet                       ->
+    HasTy E G y TySet                       ->
+    HasTy E G (Elem x y) TyProp
 | HasTyLeq : forall (G:Ctx) (x y:Term),
-    HasTy S G x TySet ->
-    HasTy S G y TySet ->
-    HasTy S G (Leq x y) TyProp
+    HasTy E G x TySet                       ->
+    HasTy E G y TySet                       ->
+    HasTy E G (Leq x y) TyProp
 | HasTyGeq : forall (G:Ctx) (x y:Term),
-    HasTy S G x TySet ->
-    HasTy S G y TySet ->
-    HasTy S G (Geq x y) TyProp
+    HasTy E G x TySet                       ->
+    HasTy E G y TySet                       ->
+    HasTy E G (Geq x y) TyProp
 | HasTyLt : forall (G:Ctx) (x y:Term),
-    HasTy S G x TySet ->
-    HasTy S G y TySet ->
-    HasTy S G (Lt x y) TyProp
+    HasTy E G x TySet                       ->
+    HasTy E G y TySet                       ->
+    HasTy E G (Lt x y) TyProp
 | HasTyGt : forall (G:Ctx) (x y:Term),
-    HasTy S G x TySet ->
-    HasTy S G y TySet ->
-    HasTy S G (Gt x y) TyProp
+    HasTy E G x TySet                       ->
+    HasTy E G y TySet                       ->
+    HasTy E G (Gt x y) TyProp
 | HasTyEqual : forall (G:Ctx) (x y:Term),
-    HasTy S G x TySet ->
-    HasTy S G y TySet ->
-    HasTy S G (Equal x y) TyProp
+    HasTy E G x TySet                       ->
+    HasTy E G y TySet                       ->
+    HasTy E G (Equal x y) TyProp
 | HasTyNotEq : forall (G:Ctx) (x y:Term),
-    HasTy S G x TySet ->
-    HasTy S G y TySet ->
-    HasTy S G (NotEq x y) TyProp
+    HasTy E G x TySet                       ->
+    HasTy E G y TySet                       ->
+    HasTy E G (NotEq x y) TyProp
 | HasTyImp : forall (G:Ctx) (p q:Term),
-    HasTy S G p TyProp ->
-    HasTy S G q TyProp ->
-    HasTy S G (Imp p q) TyProp
+    HasTy E G p TyProp                      ->
+    HasTy E G q TyProp                      ->
+    HasTy E G (Imp p q) TyProp
 | HasTyIff : forall (G:Ctx) (p q:Term),
-    HasTy S G p TyProp ->
-    HasTy S G q TyProp ->
-    HasTy S G (Iff p q) TyProp
+    HasTy E G p TyProp                      ->
+    HasTy E G q TyProp                      ->
+    HasTy E G (Iff p q) TyProp
 | HasTyAnd : forall (G:Ctx) (p q:Term),
-    HasTy S G p TyProp ->
-    HasTy S G q TyProp ->
-    HasTy S G (And p q) TyProp
+    HasTy E G p TyProp                      ->
+    HasTy E G q TyProp                      ->
+    HasTy E G (And p q) TyProp
 | HasTyOr : forall (G:Ctx) (p q:Term),
-    HasTy S G p TyProp ->
-    HasTy S G q TyProp ->
-    HasTy S G (Or p q) TyProp
+    HasTy E G p TyProp                      ->
+    HasTy E G q TyProp                      ->
+    HasTy E G (Or p q) TyProp
 | HasTyNot : forall (G:Ctx) (p:Term),
-    HasTy S G p TyProp ->
-    HasTy S G (Not p) TyProp
+    HasTy E G p TyProp                      ->
+    HasTy E G (Not p) TyProp
 | HasTyAll : forall (G:Ctx) (vty:VarTy) (p:Term),
-    HasTy S (toTy vty :: G) p TyProp ->
-    HasTy S G (All vty p) TyProp
+    HasTy E (toTy vty :: G) p TyProp        ->
+    HasTy E G (All vty p) TyProp
 | HasTyEx : forall (G:Ctx) (vty:VarTy) (p:Term),
-    HasTy S (toTy vty :: G) p TyProp ->
-    HasTy S G (Ex vty p) TyProp
+    HasTy E (toTy vty :: G) p TyProp        ->
+    HasTy E G (Ex vty p) TyProp
 | HasTyThe : forall (G:Ctx) (p:Term),
-    HasTy S (TySet :: G) p TyProp ->
-    HasTy S G (The p) TySet
+    HasTy E (TySet :: G) p TyProp           ->
+    HasTy E G (The p) TySet
 | HasTyLam : forall (G:Ctx) (p:Term),
-    HasTy S (TySet :: G) p TyProp ->
-    HasTy S G (Lam p) TyClass
+    HasTy E (TySet :: G) p TyProp           ->
+    HasTy E G (Lam p) TyClass
 | HasTyApp : forall (G:Ctx) (A x:Term),
-    HasTy S G A TyClass ->
-    HasTy S G x TySet ->
-    HasTy S G (App A x) TyProp
-with HasTys (S:Sigs) : Ctx -> list Term -> list Ty -> Prop :=
+    HasTy E G A TyClass                     ->
+    HasTy E G x TySet                       ->
+    HasTy E G (App A x) TyProp
+with HasTys (E:Env) : Ctx -> list Term -> list Ty -> Prop :=
 | HasTysNil : forall (G:Ctx),
-    HasTys S G [] []
-| HasTysCons : forall (G:Ctx) (t:Term) (ts:list Term) (ty:Ty)
-    (tys:list Ty),
-    HasTy S G t ty ->
-    HasTys S G ts tys ->
-    HasTys S G (t :: ts) (ty :: tys)
+    HasTys E G [] []
+| HasTysCons : forall (G:Ctx) (t:Term) (ts:list Term) (ty:Ty) (tys:list Ty),
+    HasTy E G t ty                          ->
+    HasTys E G ts tys                       ->
+    HasTys E G (t :: ts) (ty :: tys)
 .
