coq/ZF/Meta/HasTyIn.v
@@ -1,9 +1,0 @@
-Require Import ZF.Meta.Ctx.
-Require Import ZF.Meta.Env.
-Require Import ZF.Meta.Term.HasTy.
-Require Import ZF.Meta.Term.Syntax.
-Require Import ZF.Meta.Ty.
-
-(* A term is well typed in an environment through its signatures view.          *)
-Definition HasTyIn (e:Env) (G:Ctx) (t:Term) (ty:Ty) : Prop :=
-  HasTy (Env.toSigs e) G t ty.
