coq/ZF/Meta/Term/HasTyDecl.v
@@ -5,6 +5,6 @@ Require Import ZF.Meta.Term.HasTy.
 (* A term declaration is well typed when its body has its declared sort.        *)
 Definition HasTyDecl (e:Env) (d:Decl) : Prop :=
   match Term.Decl.body d with
-  | Some t => HasTy (Env.toSigs e) (Term.Decl.ctx d) t (Term.Decl.res d)
+  | Some t => HasTy e (Term.Decl.ctx d) t (Term.Decl.res d)
   | None   => True
   end.
