coq/ZF/Meta/Test/Axiom/Choice.v
@@ -6,7 +6,6 @@ Require Import ZF.Meta.Term.Decl.
 Require Import ZF.Meta.Env.
 Require Import ZF.Meta.Term.Syntax.
 Require Import ZF.Meta.Term.HasTy.
-Require Import ZF.Meta.HasTyIn.
 Require Import ZF.Meta.Ty.
 
 Import ListNotations.
@@ -47,11 +46,11 @@ Definition Choice : Term :=
               (Elem (Ident "eval" [Var 1; Var 0]) (Var 0))))))).
 
 (* The choice example is a proposition in the local test environment.           *)
-Proposition HasTy : HasTyIn env Ctx.empty Choice TyProp.
+Proposition HasTy : HasTy env Ctx.empty Choice TyProp.
 Proof.
   (* Proof by Hermes + gpt 5.5                                                  *)
   apply HasTyAll, HasTyEx, HasTyAnd.
-  - apply HasTyIdent with (argTys := [TySet; TySet]). 1: reflexivity.
+  - apply HasTyIdent with [TySet; TySet]. 1: reflexivity.
     apply HasTysCons.
     + apply (HasTyVar _ _ _ TySet). reflexivity.
     + apply HasTysCons.
@@ -62,10 +61,10 @@ Proof.
     + apply HasTyImp.
       * apply HasTyNotEq.
         -- apply (HasTyVar _ _ _ TySet). reflexivity.
-        -- apply HasTyIdent with (argTys := []). 1: reflexivity.
+        -- apply HasTyIdent with []. 1: reflexivity.
            apply HasTysNil.
       * apply HasTyElem.
-        -- apply HasTyIdent with (argTys := [TySet; TySet]). 1: reflexivity.
+        -- apply HasTyIdent with [TySet; TySet]. 1: reflexivity.
            apply HasTysCons.
            ++ apply (HasTyVar _ _ _ TySet). reflexivity.
            ++ apply HasTysCons.
