coq/ZF/Meta/Test/Axiom/Foundation.v
@@ -6,7 +6,6 @@ Require Import ZF.Meta.Term.Decl.
 Require Import ZF.Meta.Env.
 Require Import ZF.Meta.Term.Syntax.
 Require Import ZF.Meta.Term.HasTy.
-Require Import ZF.Meta.HasTyIn.
 Require Import ZF.Meta.Ty.
 
 Import ListNotations.
@@ -39,23 +38,23 @@ Definition Foundation : Term :=
             (Ident "empty" []))))).
 
 (* The foundation example is a proposition in the local test environment.       *)
-Proposition HasTy : HasTyIn env Ctx.empty Foundation TyProp.
+Proposition HasTy : HasTy env Ctx.empty Foundation TyProp.
 Proof.
   (* Proof by Hermes + gpt 5.5                                                  *)
   apply HasTyAll, HasTyImp.
   - apply HasTyNotEq.
     + apply (HasTyVar _ _ _ TySet). reflexivity.
-    + apply HasTyIdent with (argTys := []). 1: reflexivity.
+    + apply HasTyIdent with []. 1: reflexivity.
       apply HasTysNil.
   - apply HasTyEx, HasTyAnd.
     + apply HasTyElem; apply (HasTyVar _ _ _ TySet); reflexivity.
     + apply HasTyEqual.
-      * apply HasTyIdent with (argTys := [TySet; TySet]). 1: reflexivity.
+      * apply HasTyIdent with [TySet; TySet]. 1: reflexivity.
         apply HasTysCons.
         -- apply (HasTyVar _ _ _ TySet). reflexivity.
         -- apply HasTysCons.
            ++ apply (HasTyVar _ _ _ TySet). reflexivity.
            ++ apply HasTysNil.
-      * apply HasTyIdent with (argTys := []). 1: reflexivity.
+      * apply HasTyIdent with []. 1: reflexivity.
         apply HasTysNil.
 Qed.
