coq/ZF/Meta/Test/Axiom/NonEmptyUniverse.v
@@ -2,7 +2,6 @@ Require Import ZF.Meta.Ctx.
 Require Import ZF.Meta.Env.
 Require Import ZF.Meta.Term.Syntax.
 Require Import ZF.Meta.Term.HasTy.
-Require Import ZF.Meta.HasTyIn.
 Require Import ZF.Meta.Ty.
 
 (* exists x, True                                                               *)
@@ -10,7 +9,7 @@ Definition NonEmptyUniverse : Term :=
   Ex VarTySet Top.
 
 (* The non-empty-universe example is a proposition in the empty environment.    *)
-Proposition HasTy : HasTyIn Env.empty Ctx.empty NonEmptyUniverse TyProp.
+Proposition HasTy : HasTy Env.empty Ctx.empty NonEmptyUniverse TyProp.
 Proof.
   (* Proof by Hermes + gpt 5.5                                                  *)
   apply HasTyEx, HasTyTop.
