coq/ZF/Meta/Test/Axiom/Pairing.v
@@ -2,7 +2,6 @@ Require Import ZF.Meta.Ctx.
 Require Import ZF.Meta.Env.
 Require Import ZF.Meta.Term.Syntax.
 Require Import ZF.Meta.Term.HasTy.
-Require Import ZF.Meta.HasTyIn.
 Require Import ZF.Meta.Ty.
 
 (* forall a b, exists c, forall x, x :< c <-> x = a \/ x = b                    *)
@@ -18,7 +17,7 @@ Definition Pairing : Term :=
               (Equal (Var 0) (Var 2))))))).
 
 (* The pairing example is a proposition in the empty environment.               *)
-Proposition PairingCheck : HasTyIn Env.empty Ctx.empty Pairing TyProp.
+Proposition PairingCheck : HasTy Env.empty Ctx.empty Pairing TyProp.
 Proof.
   (* Proof by Hermes + gpt 5.5                                                  *)
   apply HasTyAll, HasTyAll, HasTyEx, HasTyAll, HasTyIff.
