coq/ZF/Meta/Test/Axiom/Power.v
@@ -2,7 +2,6 @@ Require Import ZF.Meta.Ctx.
 Require Import ZF.Meta.Env.
 Require Import ZF.Meta.Term.Syntax.
 Require Import ZF.Meta.Term.HasTy.
-Require Import ZF.Meta.HasTyIn.
 Require Import ZF.Meta.Ty.
 
 (* forall a, exists b, forall x, x :< b <-> x <= a                              *)
@@ -15,7 +14,7 @@ Definition Power : Term :=
           (Leq (Var 0) (Var 2))))).
 
 (* The power example is a proposition in the empty environment.                 *)
-Proposition HasTy : HasTyIn Env.empty Ctx.empty Power TyProp.
+Proposition HasTy : HasTy Env.empty Ctx.empty Power TyProp.
 Proof.
   (* Proof by Hermes + gpt 5.5                                                  *)
   apply HasTyAll, HasTyEx, HasTyAll, HasTyIff.
