coq/ZF/Meta/Test/Axiom/Specification.v
@@ -2,7 +2,6 @@ Require Import ZF.Meta.Ctx.
 Require Import ZF.Meta.Env.
 Require Import ZF.Meta.Term.Syntax.
 Require Import ZF.Meta.Term.HasTy.
-Require Import ZF.Meta.HasTyIn.
 Require Import ZF.Meta.Ty.
 
 (* forall P, forall a, exists b, forall x, x :< b <-> x :< a /\ P x             *)
@@ -18,7 +17,7 @@ Definition Specification : Term :=
               (App (Var 3) (Var 0))))))).
 
 (* The specification example is a proposition in the empty environment.         *)
-Proposition HasTy : HasTyIn Env.empty Ctx.empty Specification TyProp.
+Proposition HasTy : HasTy Env.empty Ctx.empty Specification TyProp.
 Proof.
   (* Proof by Hermes + gpt 5.5                                                  *)
   apply HasTyAll, HasTyAll, HasTyEx, HasTyAll, HasTyIff.
