coq/ZF/Meta/Test/Axiom/Union.v
@@ -2,7 +2,6 @@ Require Import ZF.Meta.Ctx.
 Require Import ZF.Meta.Env.
 Require Import ZF.Meta.Term.Syntax.
 Require Import ZF.Meta.Term.HasTy.
-Require Import ZF.Meta.HasTyIn.
 Require Import ZF.Meta.Ty.
 
 (* forall a, exists b, forall x, x :< b <-> exists y, x :< y /\ y :< a          *)
@@ -18,7 +17,7 @@ Definition Union : Term :=
               (Elem (Var 0) (Var 3))))))).
 
 (* The union example is a proposition in the empty environment.                 *)
-Proposition HasTy : HasTyIn Env.empty Ctx.empty Union TyProp.
+Proposition HasTy : HasTy Env.empty Ctx.empty Union TyProp.
 Proof.
   (* Proof by Hermes + gpt 5.5                                                  *)
   apply HasTyAll, HasTyEx, HasTyAll, HasTyIff.
