coq/ZF/Meta/Test/Class/Equiv.v
@@ -3,7 +3,6 @@ Require Import Coq.Strings.String.
 
 Require Import ZF.Meta.Ctx.
 Require Import ZF.Meta.Term.HasTy.
-Require Import ZF.Meta.HasTyIn.
 Require Import ZF.Meta.Term.Syntax.
 Require Import ZF.Meta.Ty.
 
@@ -148,11 +147,11 @@ Definition NotCompatR : Term :=
 (* Proposition typing.                                                          *)
 
 (* The reflexivity proposition is well sorted using equivalence.                *)
-Proposition ReflCheck : HasTyIn env Ctx.empty Refl TyProp.
+Proposition ReflCheck : HasTy env Ctx.empty Refl TyProp.
 Proof.
   (* Proof by Hermes + gpt 5.5                                                  *)
   apply HasTyAll.
-  apply HasTyIdent with (argTys := [TyClass; TyClass]). 1: reflexivity.
+  apply HasTyIdent with [TyClass; TyClass]. 1: reflexivity.
   apply HasTysCons.
   - apply (HasTyVar _ _ _ TyClass). reflexivity.
   - apply HasTysCons.
@@ -161,7 +160,7 @@ Proof.
 Qed.
 
 (* Equivalence compatibility is a well-sorted proposition.                      *)
-Proposition EquivCompatCheck : HasTyIn env Ctx.empty EquivCompat TyProp.
+Proposition EquivCompatCheck : HasTy env Ctx.empty EquivCompat TyProp.
 Proof.
   (* Proof by Hermes + gpt 5.5                                                  *)
   apply HasTyAll, HasTyAll, HasTyAll, HasTyAll, HasTyImp.
@@ -174,7 +173,7 @@ Proof.
 Qed.
 
 (* Left compatibility of equivalence is a well-sorted proposition.              *)
-Proposition EquivCompatLCheck : HasTyIn env Ctx.empty EquivCompatL TyProp.
+Proposition EquivCompatLCheck : HasTy env Ctx.empty EquivCompatL TyProp.
 Proof.
   (* Proof by Hermes + gpt 5.5                                                  *)
   apply HasTyAll, HasTyAll, HasTyAll, HasTyImp.
@@ -183,7 +182,7 @@ Proof.
 Qed.
 
 (* Right compatibility of equivalence is a well-sorted proposition.             *)
-Proposition EquivCompatRCheck : HasTyIn env Ctx.empty EquivCompatR TyProp.
+Proposition EquivCompatRCheck : HasTy env Ctx.empty EquivCompatR TyProp.
 Proof.
   (* Proof by Hermes + gpt 5.5                                                  *)
   apply HasTyAll, HasTyAll, HasTyAll, HasTyImp.
@@ -192,14 +191,14 @@ Proof.
 Qed.
 
 (* Symmetry of equivalence is a well-sorted proposition.                        *)
-Proposition SymCheck : HasTyIn env Ctx.empty Sym TyProp.
+Proposition SymCheck : HasTy env Ctx.empty Sym TyProp.
 Proof.
   (* Proof by Hermes + gpt 5.5                                                  *)
   apply HasTyAll, HasTyAll, HasTyImp; apply equivCheckIdent; reflexivity.
 Qed.
 
 (* Transitivity of equivalence is a well-sorted proposition.                    *)
-Proposition TranCheck : HasTyIn env Ctx.empty Tran TyProp.
+Proposition TranCheck : HasTy env Ctx.empty Tran TyProp.
 Proof.
   (* Proof by Hermes + gpt 5.5                                                  *)
   apply HasTyAll, HasTyAll, HasTyAll, HasTyImp.
@@ -208,19 +207,19 @@ Proof.
 Qed.
 
 (* Symmetry of non-equivalence is a well-sorted proposition.                    *)
-Proposition NotSymCheck : HasTyIn env Ctx.empty NotSym TyProp.
+Proposition NotSymCheck : HasTy env Ctx.empty NotSym TyProp.
 Proof.
   (* Proof by Hermes + gpt 5.5                                                  *)
   apply HasTyAll, HasTyAll, HasTyImp; apply notEquivCheckIdent; reflexivity.
 Qed.
 
 (* Equality of sets and equivalence of their classes is well sorted.            *)
-Proposition EqualToClassCheck : HasTyIn env Ctx.empty EqualToClass TyProp.
+Proposition EqualToClassCheck : HasTy env Ctx.empty EqualToClass TyProp.
 Proof.
   (* Proof by Hermes + gpt 5.5                                                  *)
   apply HasTyAll, HasTyAll, HasTyIff.
   - apply HasTyEqual; apply (HasTyVar _ _ _ TySet); reflexivity.
-  - apply HasTyIdent with (argTys := [TyClass; TyClass]). 1: reflexivity.
+  - apply HasTyIdent with [TyClass; TyClass]. 1: reflexivity.
     apply HasTysCons.
     + apply toClassCheckIdent; reflexivity.
     + apply HasTysCons.
@@ -230,13 +229,13 @@ Qed.
 
 (* Inequality of sets and non-equivalence of their classes is well sorted.      *)
 Proposition NotEqualToClassCheck :
-  HasTyIn env Ctx.empty NotEqualToClass TyProp.
+  HasTy env Ctx.empty NotEqualToClass TyProp.
 Proof.
   (* Proof by Hermes + gpt 5.5                                                  *)
   apply HasTyAll, HasTyAll, HasTyIff.
   - apply HasTyNotEq; apply (HasTyVar _ _ _ TySet); reflexivity.
   - apply HasTyNot.
-    apply HasTyIdent with (argTys := [TyClass; TyClass]). 1: reflexivity.
+    apply HasTyIdent with [TyClass; TyClass]. 1: reflexivity.
     apply HasTysCons.
     + apply toClassCheckIdent; reflexivity.
     + apply HasTysCons.
@@ -245,7 +244,7 @@ Proof.
 Qed.
 
 (* Non-equivalence is compatible with equivalence.                              *)
-Proposition NotCompatCheck : HasTyIn env Ctx.empty NotCompat TyProp.
+Proposition NotCompatCheck : HasTy env Ctx.empty NotCompat TyProp.
 Proof.
   (* Proof by Hermes + gpt 5.5                                                  *)
   apply HasTyAll, HasTyAll, HasTyAll, HasTyAll, HasTyImp.
@@ -258,7 +257,7 @@ Proof.
 Qed.
 
 (* Non-equivalence is left-compatible with equivalence.                         *)
-Proposition NotCompatLCheck : HasTyIn env Ctx.empty NotCompatL TyProp.
+Proposition NotCompatLCheck : HasTy env Ctx.empty NotCompatL TyProp.
 Proof.
   (* Proof by Hermes + gpt 5.5                                                  *)
   apply HasTyAll, HasTyAll, HasTyAll, HasTyImp.
@@ -267,7 +266,7 @@ Proof.
 Qed.
 
 (* Non-equivalence is right-compatible with equivalence.                        *)
-Proposition NotCompatRCheck : HasTyIn env Ctx.empty NotCompatR TyProp.
+Proposition NotCompatRCheck : HasTy env Ctx.empty NotCompatR TyProp.
 Proof.
   (* Proof by Hermes + gpt 5.5                                                  *)
   apply HasTyAll, HasTyAll, HasTyAll, HasTyImp.
